Std/Data/Nat/Basic.lean
@@ -12,3 +12,6 @@ Divisibility of natural numbers. `a ∣ b` (typed as `\|`) says that
 there is some `c` such that `b = a * c`.
 -/
 instance : Dvd Nat := ⟨fun a b => ∃ c, b = a * c⟩
+
+/-- Sum of a list of natural numbers. -/
+protected def sum (l : List Nat) : Nat := l.foldr (·+·) 0
