Std/Data/Array/Lemmas.lean
@@ -41,6 +41,9 @@ attribute [simp] isEmpty uget
 @[simp] theorem get?_eq_getElem? (a : Array α) (i : Nat) : a.get? i = a[i]? := rfl
 theorem getElem_fin_eq_data_get (a : Array α) (i : Fin _) : a[i] = a.data.get i := rfl
 
+@[simp] theorem ugetElem_eq_getElem (a : Array α) {i : USize} (h : i.toNat < a.size) :
+  a[i] = a[i.toNat] := rfl
+
 theorem getElem?_eq_getElem (a : Array α) (i : Nat) (h : i < a.size) : a[i]? = a[i] :=
   getElem?_pos ..
 
