Std/Data/HashMap/Lemmas.lean
@@ -1,0 +1,120 @@
+/-
+Copyright (c) 2022 Mario Carneiro. All rights reserved.
+Released under Apache 2.0 license as described in the file LICENSE.
+Authors: Mario Carneiro
+-/
+import Std.Data.HashMap.Basic
+import Std.Data.List.Lemmas
+import Std.Data.Array.Lemmas
+import Std.Tactic.ShowTerm
+
+namespace Std.HashMap.Imp
+
+namespace Bucket
+
+@[ext] protected theorem ext : ∀ {b₁ b₂ : Bucket α β}, b₁.1.data = b₂.1.data → b₁ = b₂
+  | ⟨⟨_⟩, _⟩, ⟨⟨_⟩, _⟩, rfl => rfl
+
+theorem update_data (self : Bucket α β) (i d h) :
+    (self.update i d h).1.data = self.1.data.set i.toNat d := rfl
+
+theorem exists_of_update (self : Bucket α β) (i d h) :
+    ∃ l₁ l₂, self.1.data = l₁ ++ self.1[i] :: l₂ ∧ List.length l₁ = i.toNat ∧
+      (self.update i d h).1.data = l₁ ++ d :: l₂ := by
+  simp [Array.getElem_eq_data_get]; exact List.exists_of_set' h
+
+theorem size_eq (data : Bucket α β) :
+  size data = .sum (data.1.data.map (·.toList.length)) := rfl
+
+theorem mk_size (h) : (mk n h : Bucket α β).size = 0 := by
+  simp [Bucket.size_eq, Bucket.mk, mkArray]; clear h
+  induction n <;> simp [*]
+
+end Bucket
+
+theorem empty'_WF [BEq α] [Hashable α] : (empty' n h : Imp α β).buckets.WF := by
+  refine ⟨fun _ _ _ h => ?_, fun i h => ?_⟩
+  · simp [Bucket.mk, empty', mkArray, List.mem_replicate] at h
+    simp [h, List.Pairwise.nil]
+  · simp [Bucket.mk, empty', mkArray, Array.getElem_eq_data_get, AssocList.All]
+
+theorem reinsertAux_size (hashFn : α → UInt64) (data : Bucket α β) (a : α) (b : β) :
+    (reinsertAux hashFn data a b).size = data.size.succ := by
+  simp [Bucket.size_eq, reinsertAux]
+  refine have ⟨l₁, l₂, h₁, _, eq⟩ := Bucket.exists_of_update ..; eq ▸ ?_
+  simp [h₁, Nat.succ_add]; rfl
+
+theorem expand_size [Hashable α] {buckets : Bucket α β} :
+    (expand sz buckets).buckets.size = buckets.size := by
+  rw [expand, go]
+  · rw [Bucket.mk_size]; simp [Bucket.size]
+  · intro.
+where
+  go (i source) (target : Bucket α β) (hs : ∀ j < i, source.data.getD j .nil = .nil) :
+      (expand.go i source target).size =
+        .sum (source.data.map (·.toList.length)) + target.size := by
+    unfold expand.go; split
+    case _ H =>
+      refine (go (i+1) _ _ fun j hj => ?a).trans ?b; simp
+      case a =>
+        simp [List.getD_eq_get?, List.get?_set]; split
+        case _ => cases List.get? .. <;> rfl
+        case _ H => exact hs _ (Nat.lt_of_le_of_ne (Nat.le_of_lt_succ hj) (Ne.symm H))
+      case b =>
+        refine have ⟨l₁, l₂, h₁, _, eq⟩ := List.exists_of_set' H; eq ▸ ?_
+        simp [h₁, Bucket.size_eq]
+        rw [Nat.add_assoc, Nat.add_assoc, Nat.add_assoc]; congr 1
+        (conv => rhs; rw [Nat.add_left_comm]); congr 1
+        rw [← Array.getElem_eq_data_get]
+        have := @reinsertAux_size α β; simp [Bucket.size] at this
+        induction source[i].toList generalizing target <;> simp [*, Nat.succ_add]; rfl
+    case _ H =>
+      rw [(_ : Nat.sum _ = 0), Nat.zero_add]
+      rw [← (_ : source.data.map (fun _ => .nil) = source.data)]
+      · simp; induction source.data <;> simp [*]
+      refine List.ext_get (by simp) fun j h₁ h₂ => ?_
+      simp
+      have := (hs j (Nat.lt_of_lt_of_le h₂ (Nat.not_lt.1 H))).symm
+      rwa [List.getD_eq_get?, List.get?_eq_get, Option.getD_some] at this
+termination_by go i source _ _ => source.size - i
+
+theorem insert_size [BEq α] [Hashable α] {m : Imp α β} {k v}
+    (h : m.size = m.buckets.size) :
+    (insert m k v).size = (insert m k v).buckets.size := by
+  unfold insert; dsimp [cond]; split
+  · dsimp [Bucket.size]
+    refine have ⟨_, _, h₁, _, eq⟩ := Bucket.exists_of_update ..; eq ▸ ?_
+    simp [h, h₁, Bucket.size_eq]
+  split
+  · dsimp [Bucket.size]
+    refine have ⟨_, _, h₁, _, eq⟩ := Bucket.exists_of_update ..; eq ▸ ?_
+    simp [h, h₁, Bucket.size_eq, Nat.succ_add]; rfl
+  · rw [expand_size]; simp [h, expand, Bucket.size]
+    refine have ⟨_, _, h₁, _, eq⟩ := Bucket.exists_of_update ..; eq ▸ ?_
+    simp [h₁, Bucket.size_eq, Nat.succ_add]; rfl
+
+theorem erase_size [BEq α] [Hashable α] {m : Imp α β} {k}
+    (h : m.size = m.buckets.size) :
+    (erase m k).size = (erase m k).buckets.size := by
+  unfold erase; dsimp [cond]; split
+  case _ H =>
+    simp [h, Bucket.size]
+    refine have ⟨_, _, h₁, _, eq⟩ := Bucket.exists_of_update ..; eq ▸ ?_
+    simp [h, h₁, Bucket.size_eq]
+    rw [(_ : List.length _ = _ + 1), Nat.add_right_comm]; {rfl}
+    clear h₁ eq
+    simp [AssocList.contains_eq] at H
+    have ⟨a, h₁, h₂⟩ := H
+    refine have ⟨_, _, _, _, _, h, eq⟩ := List.exists_of_eraseP h₁ h₂; eq ▸ ?_
+    simp [h]; rfl
+  case h_2 => exact h
+
+-- TODO
+-- theorem WF_iff [BEq α] [Hashable α] {m : Imp α β} :
+--     m.WF ↔ m.size = m.buckets.size ∧ m.buckets.WF := by
+--   refine ⟨fun h => ?_, fun ⟨h₁, h₂⟩ => .mk h₁ h₂⟩
+--   induction h with
+--   | mk h₁ h₂ => exact ⟨h₁, h₂⟩
+--   | @empty' _ h => exact ⟨(Bucket.mk_size h).symm, empty'_WF⟩
+--   | insert _ ih => exact ⟨insert_size ih.1, sorry⟩
+--   | erase _ ih => exact ⟨erase_size ih.1, sorry⟩
