Std/Tactic/ShowTerm.lean
@@ -22,8 +22,10 @@ namespace Std.Tactic
 elab (name := showTermTac) tk:"show_term " t:tacticSeq : tactic => withMainContext do
   let g ← getMainGoal
   evalTactic t
-  addExactSuggestion tk /- FIXME: we'd like the range for the whole tactic -/
-    (← instantiateMVars (mkMVar g)).headBeta
+  -- TODO: At the moment it is more useful to use an Expr MessageData
+  -- instead of a Syntax because the former is clickable in the infoview
+  -- addExactSuggestion tk (← instantiateMVars (mkMVar g)).headBeta
+  logInfoAt tk (← instantiateMVars (mkMVar g)).headBeta
 
 /--
 `show_term e` elaborates `e`, then prints the generated term.
@@ -33,5 +35,8 @@ elab (name := showTermTac) tk:"show_term " t:tacticSeq : tactic => withMainConte
 elab (name := showTerm) tk:"show_term " t:term : term <= ty => do
   let e ← Term.elabTermEnsuringType t ty
   Term.synthesizeSyntheticMVarsNoPostponing
-  addTermSuggestion tk (← instantiateMVars e).headBeta
+  -- TODO: At the moment it is more useful to use an Expr MessageData
+  -- instead of a Syntax because the former is clickable in the infoview
+  -- addTermSuggestion tk (← instantiateMVars e).headBeta
+  logInfoAt tk (← instantiateMVars e).headBeta
   pure e
